\begin{answer}
We are given 
\begin{equation} \label{eq:J1}
    J(\theta) = -\frac{1}{n} \sum_{i=1}^{n} \big(
    y^{(i)}log(h_\theta(x^{(i)})) + (1-y^{(i)}) log(1 -h_\theta x^{(i)})
    \big)
\end{equation}
To find the $\nabla_\theta$J($\theta$) let's break $\nabla_\theta J(\theta)$ into two components.
Let's first consider
\begin{equation}
    \nabla_\theta \sum_{i=1}^{n} 
    y^{(i)}log(h_\theta(x^{(i)}))
\end{equation}
\begin{equation}
    =  \sum_{i=1}^{n} 
    y^{(i)} \nabla_\theta log(h_\theta(x^{(i)}))
\end{equation}
\begin{equation} \label{eq:A}
    = \sum_{i=1}^{n} y^{(i)}\frac{\nabla_{\theta}h_{\theta}(x^{(i)})}{h_{\theta}(x^{(i)})}
\end{equation}
Where 
\begin{equation} 
    \nabla_\theta h_{\theta}(x^{(i)}) = \nabla_\theta g(\theta^T x^{(i)})
\end{equation} 
Let z = $\theta^T x^{(i)}$ and recall $g'(z) = g(z)(1-g(z))$. We then solve $\nabla_\theta g(\theta^T x^{(i)})$ with this property and the chain rule.
\begin{equation} \label{eq:g}
    \nabla_\theta h_{\theta}(x^{(i)}) = g(\theta^T x^{(i)})(1-g(\theta^T x^{(i)})) x^{(i)}
\end{equation}
Substituting \ref{eq:g} into \ref{eq:A} 
\begin{equation} 
        = \sum_{i=1}^{n} y^{(i)}
        \frac{g(\theta^T x^{(i)})(1-g(\theta^T x^{(i)})) x^{(i)}}
        {g(\theta^T x^{(i)})}
\end{equation}

\begin{equation}  \label{eq:Adone}
        = \sum_{i=1}^{n} y^{(i)}
        (1-g(\theta^T x^{(i)})) x^{(i)}
\end{equation}

Next, let's consider 
\begin{equation}
     \nabla_\theta \sum_{i=1}^{n} (1-y^{(i)}) log(1 -h_\theta (x^{(i)}))
\end{equation}
\begin{equation}
     =  \sum_{i=1}^{n} (1-y^{(i)}) \nabla_\theta log(1 -h_\theta (x^{(i)}))
\end{equation}
\begin{equation}\label{eq:B}
     =  \sum_{i=1}^{n} (1-y^{(i)}) 
     \frac{ -\nabla_\theta h_\theta (x^{(i)})}
     {1 -h_\theta (x^{(i)})}
\end{equation}
Substitute \ref{eq:g} into \ref{eq:B}
\begin{equation}
     =  \sum_{i=1}^{n} (1-y^{(i)}) 
     \frac{ -g(\theta^T x^{(i)})(1-g(\theta^T x^{(i)})) x^{(i)}}
     {1 -g(\theta^T x^{(i)})}
\end{equation}
\begin{equation} \label{eq:Bdone}
     =  \sum_{i=1}^{n} (y^{(i)} - 1) g(\theta^T x^{(i)})x^{(i)}
\end{equation}
Combining \ref{eq:Adone} and \ref{eq:Bdone} back into $\nabla_\theta J(\theta)$ from \ref{eq:J1}, we have
\begin{equation}
    \nabla_\theta J(\theta) = -\frac{1}{n} \sum_{i=1}^{n} 
    \big(
    (1-g(\theta^T x^{(i)})) x^{(i)}
    + (y^{(i)} - 1) g(\theta^T x^{(i)})x^{(i)}
    \big)
\end{equation
\begin{equation}
    = -\frac{1}{n} \sum_{i=1}^{n} 
    \big(
    y^{(i)}(1-g(\theta^T x^{(i)})) x^{(i)}
    + (y^{(i)} - 1) g(\theta^T x^{(i)})x^{(i)}
    \big)
\end{equation}
\begin{equation}
    = -\frac{1}{n} \sum_{i=1}^{n} 
    \big(
    y^{(i)}x^{(i)} - y^{(i)}g(\theta^T x^{(i)})x^{(i)} +
    y^{(i)}g(\theta^T x^{(i)})x^{(i)} - g(\theta^T x^{(i)})x^{(i)}
    \big)
\end{equation}
\begin{equation}
    = -\frac{1}{n} \sum_{i=1}^{n} 
    \big(
    y^{(i)}x^{(i)} - g(\theta^T x^{(i)})x^{(i)}
    \big)
\end{equation}
\begin{equation}
    H_\theta J(\theta) 
    = -\frac{1}{n} \sum_{i=1}^{n} 
    \big(
    0 - \frac{\partial}{\partial \theta} g(\theta^T x^{(i)})x^{(i)}
    \big)
\end{equation}
\begin{equation}
    = -\frac{1}{n} \sum_{i=1}^{n} 
    -  g(\theta^T x^{(i)})(1-g(\theta^T x^{(i)})) x^{(i)} x^{(i)}T
\end{equation}
\begin{equation}
    = \frac{1}{n} \sum_{i=1}^{n} 
    g(\theta^T x^{(i)})(1-g(\theta^T x^{(i)})) x^{(i)} x^{(i)}T
\end{equation}
Finally, we need to show that the hessian is a PSD for any vector z where $z= \theta^Tx$,  $h_\theta (x^{(i)}) = g(\theta^T x^{(i)})$ and $g(z) = \frac{1}{1+exp(-z)}$. So we need to show that the below is a PSD.
\begin{equation}
    z_\theta^T H_\theta J(\theta)z= z^T \frac{1}{n} \sum_{i=1}^{n} 
    g(\theta^T x^{(i)})(1-g(\theta^T x^{(i)})) x^{(i)} x^{(i)}T z
\end{equation}

We know that $g(\theta^T x^{(i)}) = h_\theta (x^{(i)})$ and that the hypothesis function of classifiers outputs probabilities between 0 to 1. Thus
\begin{equation}
    0 \leq g(\theta^T x^{(i)})(1-g(\theta^T x^{(i)})) \leq   1
\end{equation}
We then have a scalar component, C in the below
\begin{equation}
    z_\theta^T H_\theta J(\theta)z= z^T \frac{1}{n} \sum_{i=1}^{n} 
    C x^{(i)} x^{(i)}T z
\end{equation}
\begin{equation}
    z_\theta^T H_\theta J(\theta)z = \frac{1}{n} \sum_{i=1}^{n} 
    C  z^T x^{(i)} x^{(i)}T z  = \frac{1}{n} \sum_{i=1}^{n} 
    C  (z^T x^{(i)})^2 
\end{equation}
Squares are always non-negative and \textit{n} in the summation is greater or equal to 1 for a non-trivial solution. Therefore, $H_\theta J(\theta)$ is a PSD.


\end{answer}
